feat: redefine `String`, part two (#10457)
This PR introduces safe alternatives to `String.Pos` and `Substring`
that can only represent valid positions/slices.

Specifically, the PR

- introduces the predicate `String.Pos.IsValid`;
- proves several nontrivial equivalent conditions for
`String.Pos.IsValid`;
- introduces `String.ValidPos`, which is a `String.Pos` with an
`IsValid` proof;
- introduces `String.Slice`, which is like `Substring` but made from
`String.ValidPos` instead of `Pos`;
- introduces `String.Pos.IsValidForSlice`, which is like
`String.Pos.IsValid` but for slices;
- introduces `String.Slice.Pos`, which is like `String.ValidPos` but for
slices;
- introduces various functions for converting between the two types of
positions.

The API added in this PR is not complete. It will be expanded in future
PRs with addional operations and verification.

src/Init/Data/String/Basic.lean
@@ -33,6 +33,10 @@ theorem List.utf8Encode_append {l l' : List Char} :
 theorem List.utf8Encode_cons {c : Char} {l : List Char} : (c :: l).utf8Encode = [c].utf8Encode ++ l.utf8Encode := by
   rw [← singleton_append, List.utf8Encode_append]
 
+theorem List.isUtf8FirstByte_getElem_utf8Encode_singleton {c : Char} {i : Nat} {hi : i < [c].utf8Encode.size} :
+    UInt8.IsUtf8FirstByte [c].utf8Encode[i] ↔ i = 0 := by
+  simp [List.utf8Encode_singleton, UInt8.isUtf8FirstByte_getElem_utf8EncodeChar]
+
 @[simp]
 theorem String.utf8EncodeChar_ne_nil {c : Char} : String.utf8EncodeChar c ≠ [] := by
   fun_cases String.utf8EncodeChar with simp
@@ -73,7 +77,7 @@ theorem ByteArray.isValidUtf8_utf8Encode_singleton_append_iff {b : ByteArray} {c
       ByteArray.append_right_inj] at hl
     exact hl ▸ isValidUtf8_utf8Encode
 
-@[expose]
+@[inline, expose]
 def ByteArray.utf8Decode? (b : ByteArray) : Option (Array Char) :=
   go (b.size + 1) 0 #[] (by simp) (by simp)
 where
@@ -220,7 +224,7 @@ Examples:
 * `"abc".length = 3`
 * `"L∃∀N".length = 4`
 -/
-@[extern "lean_string_length"]
+@[extern "lean_string_length", expose]
 def String.length (b : @& String) : Nat :=
   b.data.length
 
@@ -282,7 +286,7 @@ theorem ByteArray.utf8Decode?_utf8Encode_singleton_append {l : ByteArray} {c : C
     simp only [List.push_toArray, List.nil_append, Nat.zero_add]
     congr 1
     apply ByteArray.utf8Decode?.go.congr _ rfl rfl
-    apply extract_append_eq_right
+    apply extract_append_eq_right _ (by simp)
     simp [List.utf8Encode_singleton]
 
 @[simp]
@@ -406,6 +410,19 @@ instance (p₁ p₂ : String.Pos) : Decidable (LT.lt p₁ p₂) :=
 instance : Min String.Pos := minOfLe
 instance : Max String.Pos := maxOfLe
 
+theorem Pos.le_iff {i₁ i₂ : Pos} : i₁ ≤ i₂ ↔ i₁.byteIdx ≤ i₂.byteIdx := .rfl
+
+theorem Pos.lt_iff {i₁ i₂ : Pos} : i₁ < i₂ ↔ i₁.byteIdx < i₂.byteIdx := .rfl
+
+@[simp]
+theorem byteIdx_endPos {s : String} : s.endPos.byteIdx = s.utf8ByteSize := rfl
+
+@[simp]
+theorem utf8ByteSize_ofByteArray {b : ByteArray} {h} :
+    (String.ofByteArray b h).utf8ByteSize = b.size := rfl
+
+attribute [ext] String.Pos
+
 instance : LT String :=
   ⟨fun s₁ s₂ => s₁.data < s₂.data⟩
 
@@ -429,17 +446,303 @@ instance decLE (s₁ s₂ : String) : Decidable (s₁ ≤ s₂) :=
 /--
 Converts a string to a list of characters.
 
-Even though the logical model of strings is as a structure that wraps a list of characters, this
-operation takes time and space linear in the length of the string. At runtime, strings are
-represented as dynamic arrays of bytes.
+Since strings are represented as dynamic arrays of bytes containing the string encoded using
+UTF-8, this operation takes time and space linear in the length of the string.
 
 Examples:
  * `"abc".toList = ['a', 'b', 'c']`
  * `"".toList = []`
  * `"\n".toList = ['\n']`
 -/
+@[inline, expose]
 def toList (s : String) : List Char :=
   s.data
+
+/--
+Predicate for validity of positions inside a `String`.
+
+There are multiple equivalent definitions for validity.
+
+We say that a position is valid if the string obtained by taking all of the bytes up to, but
+excluding, the given position, is valid UTF-8; see `Pos.isValid_iff_isValidUtf8_extract_zero`.
+
+Similarly, a position is valid if the string obtained by taking all of the bytes starting at the
+given position is valid UTF-8; see `Pos.isValid_iff_isValidUtf8_extract_utf8ByteSize`.
+
+An equivalent condition is that the position is the length of the UTF-8 encoding of
+some prefix of the characters of the string; see `Pos.isValid_iff_exists_append` and
+`Pos.isValid_iff_exists_take_data`.
+
+Another equivalent condition that can be checked efficiently is that the position is either the
+end position or strictly smaller than the end position and the byte at the position satisfies
+`UInt8.IsUtf8FirstByte`; see `Pos.isValid_iff_isUtf8FirstByte`.
+
+Examples:
+ * `String.Pos.IsValid "abc" ⟨0⟩`
+ * `String.Pos.IsValid "abc" ⟨1⟩`
+ * `String.Pos.IsValid "abc" ⟨3⟩`
+ * `¬ String.Pos.IsValid "abc" ⟨4⟩`
+ * `String.Pos.IsValid "𝒫(A)" ⟨0⟩`
+ * `¬ String.Pos.IsValid "𝒫(A)" ⟨1⟩`
+ * `¬ String.Pos.IsValid "𝒫(A)" ⟨2⟩`
+ * `¬ String.Pos.IsValid "𝒫(A)" ⟨3⟩`
+ * `String.Pos.IsValid "𝒫(A)" ⟨4⟩`
+-/
+structure Pos.IsValid (s : String) (off : String.Pos) : Prop where private mk ::
+  le_endPos : off ≤ s.endPos
+  isValidUtf8_extract_zero : (s.bytes.extract 0 off.byteIdx).IsValidUtf8
+
+theorem _root_.List.isPrefix_of_utf8Encode_append_eq_utf8Encode {l m : List Char} (b : ByteArray)
+    (h : l.utf8Encode ++ b = m.utf8Encode) : l <+: m := by
+  induction l generalizing m with
+  | nil => simp
+  | cons c l ih =>
+    replace h := congrArg ByteArray.utf8Decode? h
+    rw [List.utf8Decode?_utf8Encode] at h
+    rw [← List.singleton_append, List.utf8Encode_append, ByteArray.append_assoc,
+      ByteArray.utf8Decode?_utf8Encode_singleton_append] at h
+    suffices ∃ m', m = [c] ++ m' ∧ l.utf8Encode ++ b = m'.utf8Encode by
+      obtain ⟨m', rfl, hm'⟩ := this
+      simpa using ih hm'
+    have hx : (l.utf8Encode ++ b).utf8Decode?.isSome := by
+      exact Option.isSome_map ▸ Option.isSome_of_eq_some h
+    refine ⟨(l.utf8Encode ++ b).utf8Decode?.get hx |>.toList, ?_, by simp⟩
+    exact List.toArray_inj (Option.some_inj.1 (by simp [← h]))
+
+open List in
+theorem Pos.IsValid.exists {s : String} {p : Pos} (h : p.IsValid s) :
+    ∃ m₁ m₂ : List Char, m₁.utf8Encode = s.bytes.extract 0 p.byteIdx ∧ (m₁ ++ m₂).asString = s := by
+  obtain ⟨l, hl⟩ := s.isValidUtf8
+  obtain ⟨m₁, hm₁⟩ := h.isValidUtf8_extract_zero
+  suffices m₁ <+: l by
+    obtain ⟨m₂, rfl⟩ := this
+    refine ⟨m₁, m₂, hm₁.symm, ?_⟩
+    apply String.bytes_inj.1
+    simpa using hl.symm
+  apply List.isPrefix_of_utf8Encode_append_eq_utf8Encode (s.bytes.extract p.byteIdx s.bytes.size)
+  rw [← hl, ← hm₁, ← ByteArray.extract_eq_extract_append_extract _ (by simp),
+    ByteArray.extract_zero_size]
+  simpa using h.le_endPos
+
+theorem Pos.IsValid.isValidUtf8_extract_utf8ByteSize {s : String} {p : Pos} (h : p.IsValid s) :
+    ByteArray.IsValidUtf8 (s.bytes.extract p.byteIdx s.utf8ByteSize) := by
+  obtain ⟨m₁, m₂, hm, rfl⟩ := h.exists
+  simp only [List.asString_append, bytes_append, List.bytes_asString]
+  rw [ByteArray.extract_append_eq_right]
+  · exact ByteArray.isValidUtf8_utf8Encode
+  · rw [hm]
+    simp only [List.asString_append, bytes_append, List.bytes_asString, ByteArray.size_extract,
+      ByteArray.size_append, Nat.sub_zero]
+    refine (Nat.min_eq_left ?_).symm
+    simpa [utf8ByteSize, Pos.le_iff] using h.le_endPos
+  · simp [utf8ByteSize]
+
+theorem Pos.isValid_iff_exists_append {s : String} {p : Pos} :
+    p.IsValid s ↔ ∃ s₁ s₂ : String, s = s₁ ++ s₂ ∧ p = s₁.endPos := by
+  refine ⟨fun h => ⟨⟨_, h.isValidUtf8_extract_zero⟩, ⟨_, h.isValidUtf8_extract_utf8ByteSize⟩, ?_, ?_⟩, ?_⟩
+  · apply String.bytes_inj.1
+    have := Pos.le_iff.1 h.le_endPos
+    simp_all [← size_bytes]
+  · have := byteIdx_endPos ▸ Pos.le_iff.1 h.le_endPos
+    apply String.Pos.ext
+    simp [Nat.min_eq_left this]
+  · rintro ⟨s₁, s₂, rfl, rfl⟩
+    refine ⟨by simp [Pos.le_iff], ?_⟩
+    simpa [ByteArray.extract_append_eq_left] using s₁.isValidUtf8
+
+@[simp]
+theorem Pos.byteIdx_zero : (0 : Pos).byteIdx = 0 := rfl
+
+@[simp]
+theorem Pos.isValid_zero {s : String} : (0 : Pos).IsValid s where
+  le_endPos := by simp [Pos.le_iff]
+  isValidUtf8_extract_zero := by simp
+
+@[simp]
+theorem Pos.isValid_endPos {s : String} : s.endPos.IsValid s where
+  le_endPos := by simp [Pos.le_iff]
+  isValidUtf8_extract_zero := by simp [← size_bytes, s.isValidUtf8]
+
+@[simp]
+theorem Pos.isValid_empty_iff {p : Pos} : p.IsValid "" ↔ p = 0 := by
+  refine ⟨?_, ?_⟩
+  · rintro ⟨h₁, h₂⟩
+    simp only [le_iff, byteIdx_endPos, utf8ByteSize_empty, Nat.le_zero_eq] at h₁
+    ext
+    omega
+  · rintro rfl
+    simp
+
+theorem Pos.isValid_asString {l : List Char} {p : Pos} :
+    p.IsValid l.asString ↔ ∃ i, p.byteIdx = (l.take i).asString.utf8ByteSize := by
+  rw [isValid_iff_exists_append]
+  refine ⟨?_, ?_⟩
+  · rintro ⟨t₁, t₂, ht, rfl⟩
+    refine ⟨t₁.length, ?_⟩
+    have := congrArg String.data ht
+    simp only [List.data_asString, String.data_append] at this
+    simp [this]
+  · rintro ⟨i, hi⟩
+    refine ⟨(l.take i).asString, (l.drop i).asString, ?_, ?_⟩
+    · simp [← List.asString_append]
+    · simpa [Pos.ext_iff]
+
+theorem Pos.isValid_iff_exists_take_data {s : String} {p : Pos} :
+    p.IsValid s ↔ ∃ i, p.byteIdx = (s.data.take i).asString.utf8ByteSize := by
+  obtain ⟨l, rfl⟩ := s.exists_eq_asString
+  simp [isValid_asString]
+
+@[simp]
+theorem bytes_singleton {c : Char} : (String.singleton c).bytes = [c].utf8Encode := by
+  simp [singleton]
+
+theorem singleton_eq_asString {c : Char} : String.singleton c = [c].asString := by
+  simp [← String.bytes_inj]
+
+@[simp]
+theorem utf8ByteSize_singleton {c : Char} : (String.singleton c).utf8ByteSize = c.utf8Size := by
+  simp [← size_bytes, List.utf8Encode_singleton]
+
+@[simp]
+theorem Pos.isValid_singleton {c : Char} {p : Pos} :
+    p.IsValid (String.singleton c) ↔ p = 0 ∨ p.byteIdx = c.utf8Size := by
+  rw [singleton_eq_asString, Pos.isValid_asString]
+  refine ⟨?_, ?_⟩
+  · rintro ⟨i, hi'⟩
+    obtain ⟨rfl, hi⟩ : i = 0 ∨ 1 ≤ i := by omega
+    · simp [Pos.ext_iff, hi']
+    · rw [hi', List.take_of_length_le (by simpa)]
+      simp [← singleton_eq_asString]
+  · rintro (rfl|hi)
+    · exact ⟨0, by simp⟩
+    · exact ⟨1, by simp [hi, ← singleton_eq_asString]⟩
+
+@[simp]
+theorem Pos.byteIdx_sub {p₁ p₂ : Pos} : (p₁ - p₂).byteIdx = p₁.byteIdx - p₂.byteIdx := rfl
+
+@[simp]
+theorem Pos.byteIdx_add {p₁ p₂ : Pos} : (p₁ + p₂).byteIdx = p₁.byteIdx + p₂.byteIdx := rfl
+
+@[simp]
+theorem Pos.byteIdx_addChar {p : Pos} {c : Char} : (p + c).byteIdx = p.byteIdx + c.utf8Size := rfl
+
+theorem Pos.isValid_append {s t : String} {p : Pos} :
+    p.IsValid (s ++ t) ↔ p.IsValid s ∨ (s.endPos ≤ p ∧ (p - s.endPos).IsValid t) := by
+  obtain ⟨s, rfl⟩ := exists_eq_asString s
+  obtain ⟨t, rfl⟩ := exists_eq_asString t
+  rw [← List.asString_append, Pos.isValid_asString, Pos.isValid_asString, Pos.isValid_asString]
+  refine ⟨?_, ?_⟩
+  · rintro ⟨j, hj⟩
+    by_cases h : j ≤ s.length
+    · exact Or.inl ⟨j, by simp [hj, List.take_append_of_le_length h]⟩
+    · refine Or.inr ⟨?_, ⟨j - s.length, ?_⟩⟩
+      · simp [Pos.le_iff, hj, List.take_append, List.take_of_length_le (i := j) (l := s) (by omega)]
+      · simp [hj, List.take_append, List.take_of_length_le (i := j) (l := s) (by omega)]
+  · rintro (⟨j, hj⟩|⟨h, ⟨j, hj⟩⟩)
+    · refine ⟨min j s.length, ?_⟩
+      rw [List.take_append_of_le_length (Nat.min_le_right ..), ← List.take_eq_take_min, hj]
+    · refine ⟨s.length + j, ?_⟩
+      simp only [Pos.byteIdx_sub, byteIdx_endPos, Pos.le_iff] at hj h
+      simp only [List.take_append, List.take_of_length_le (i := s.length + j) (l := s) (by omega),
+        Nat.add_sub_cancel_left, List.asString_append, utf8ByteSize_append]
+      omega
+
+theorem Pos.IsValid.append_left {t : String} {p : Pos} (h : p.IsValid t) (s : String) :
+    (s.endPos + p).IsValid (s ++ t) :=
+  isValid_append.2 (Or.inr ⟨by simp [Pos.le_iff], by
+    suffices p = s.endPos + p - s.endPos by simp [← this, h]
+    simp [Pos.ext_iff]⟩)
+
+theorem Pos.IsValid.append_right {s : String} {p : Pos} (h : p.IsValid s) (t : String) :
+    p.IsValid (s ++ t) :=
+  isValid_append.2 (Or.inl h)
+
+@[simp]
+theorem append_singleton {s : String} {c : Char} : s ++ singleton c = s.push c := by
+  simp [← bytes_inj]
+
+theorem Pos.isValid_push {s : String} {c : Char} {p : Pos} :
+    p.IsValid (s.push c) ↔ p.IsValid s ∨ p = s.endPos + c := by
+  rw [← append_singleton, isValid_append, isValid_singleton]
+  simp only [le_iff, byteIdx_endPos, Pos.ext_iff, byteIdx_sub, byteIdx_zero, byteIdx_addChar]
+  refine ⟨?_, ?_⟩
+  · rintro (h|⟨h₁,(h₂|h₂)⟩)
+    · exact Or.inl h
+    · suffices p = s.endPos by simp [this]
+      simp only [Pos.ext_iff, byteIdx_endPos]
+      omega
+    · omega
+  · rintro (h|h)
+    · exact Or.inl h
+    · omega
+
+@[simp]
+theorem utf8ByteSize_push {s : String} {c : Char} :
+    (s.push c).utf8ByteSize = s.utf8ByteSize + c.utf8Size := by
+  simp [← size_bytes, List.utf8Encode_singleton]
+
+theorem endPos_push {s : String} {c : Char} : (s.push c).endPos = s.endPos + c := by
+  simp [Pos.ext_iff]
+
+theorem push_induction (s : String) (motive : String → Prop) (empty : motive "")
+    (push : ∀ b c, motive b → motive (b.push c)) : motive s := by
+  obtain ⟨m, rfl⟩ := s.exists_eq_asString
+  apply append_singleton_induction m (motive ·.asString)
+  · simpa
+  · intro l c hl
+    rw [List.asString_append, ← singleton_eq_asString, append_singleton]
+    exact push _ _ hl
+where
+  append_singleton_induction (l : List Char) (motive : List Char → Prop) (nil : motive [])
+      (append_singleton : ∀ l a, motive l → motive (l ++ [a])) : motive l := by
+    rw [← l.reverse_reverse]
+    generalize l.reverse = m
+    induction m with
+    | nil => simpa
+    | cons a m ih =>
+      rw [List.reverse_cons]
+      exact append_singleton _ _ ih
+
+/--
+Accesses the indicated byte in the UTF-8 encoding of a string.
+
+At runtime, this function is implemented by efficient, constant-time code.
+-/
+@[extern "lean_string_get_byte_fast", expose]
+def getUtf8Byte (s : @& String) (p : Pos) (h : p < s.endPos) : UInt8 :=
+  s.bytes[p.byteIdx]
+
+@[simp]
+theorem endPos_empty : "".endPos = 0 := rfl
+
+theorem Pos.isValid_iff_isUtf8FirstByte {s : String} {p : Pos} :
+    p.IsValid s ↔ p = s.endPos ∨ ∃ (h : p < s.endPos), (s.getUtf8Byte p h).IsUtf8FirstByte := by
+  induction s using push_induction with
+  | empty => simp [Pos.lt_iff]
+  | push s c ih =>
+    rw [isValid_push, ih]
+    refine ⟨?_, ?_⟩
+    · rintro ((rfl|⟨h, hb⟩)|h)
+      · refine Or.inr ⟨by simp [Pos.lt_iff, Char.utf8Size_pos], ?_⟩
+        simp only [getUtf8Byte, bytes_push, byteIdx_endPos]
+        rw [ByteArray.getElem_append_right (by simp)]
+        simp [List.isUtf8FirstByte_getElem_utf8Encode_singleton]
+      · refine Or.inr ⟨by simp [lt_iff] at h ⊢; omega, ?_⟩
+        simp only [getUtf8Byte, bytes_push]
+        rwa [ByteArray.getElem_append_left, ← getUtf8Byte]
+      · exact Or.inl (by simpa [endPos_push])
+    · rintro (h|⟨h, hb⟩)
+      · exact Or.inr (by simpa [endPos_push] using h)
+      · simp only [getUtf8Byte, bytes_push] at hb
+        by_cases h' : p < s.endPos
+        · refine Or.inl (Or.inr ⟨h', ?_⟩)
+          rwa [ByteArray.getElem_append_left h', ← getUtf8Byte] at hb
+        · refine Or.inl (Or.inl ?_)
+          rw [ByteArray.getElem_append_right (by simp [lt_iff] at h' ⊢; omega)] at hb
+          simp only [size_bytes, List.isUtf8FirstByte_getElem_utf8Encode_singleton] at hb
+          ext
+          simp only [lt_iff, byteIdx_endPos, Nat.not_lt] at ⊢ h'
+          omega
 
 /--
 Returns `true` if `p` is a valid UTF-8 position in the string `s`.
@@ -458,14 +761,1200 @@ Examples:
  * `String.Pos.isValid "𝒫(A)" ⟨3⟩ = false`
  * `String.Pos.isValid "𝒫(A)" ⟨4⟩ = true`
 -/
-@[extern "lean_string_is_valid_pos"]
+@[extern "lean_string_is_valid_pos", expose]
 def Pos.isValid (s : @&String) (p : @& Pos) : Bool :=
-  go s.data 0
-where
-  go : List Char → Pos → Bool
-  | [],    i => i = p
-  | c::cs, i => if i = p then true else go cs (i + c)
+  if h : p < s.endPos then
+    (s.getUtf8Byte p h).IsUtf8FirstByte
+  else
+    p = s.endPos
 
+@[simp]
+theorem Pos.isValid_eq_true_iff {s : String} {p : Pos} : p.isValid s = true ↔ p.IsValid s := by
+  rw [isValid_iff_isUtf8FirstByte]
+  fun_cases isValid s p with
+  | case1 h =>
+    simp_all only [decide_eq_true_eq, exists_true_left, iff_or_self]
+    rintro rfl
+    simp [lt_iff] at h
+  | case2 => simp_all
+
+@[simp]
+theorem Pos.isValid_eq_false_iff {s : String} {p : Pos} : p.isValid s = false ↔ ¬ p.IsValid s := by
+  rw [← Bool.not_eq_true, Pos.isValid_eq_true_iff]
+
+instance {s : String} {p : Pos} : Decidable (p.IsValid s) :=
+  decidable_of_iff (p.isValid s = true) Pos.isValid_eq_true_iff
+
+theorem Pos.isValid_iff_isSome_utf8DecodeChar? {s : String} {p : Pos} :
+    p.IsValid s ↔ p = s.endPos ∨ (s.bytes.utf8DecodeChar? p.byteIdx).isSome := by
+  refine ⟨?_, fun h => h.elim (by rintro rfl; simp) (fun h => ?_)⟩
+  · induction s using push_induction with
+    | empty => simp [ByteArray.utf8DecodeChar?]
+    | push s c ih =>
+      simp only [isValid_push, bytes_push]
+      refine ?_ ∘ Or.imp_left ih
+      rintro ((rfl|h)|rfl)
+      · rw [ByteArray.utf8DecodeChar?_eq_utf8DecodeChar?_extract, ByteArray.extract_append_eq_right (by simp) (by simp)]
+        simp
+      · exact Or.inr (ByteArray.isSome_utf8DecodeChar?_append h _)
+      · simp [endPos_push]
+  · refine isValid_iff_isUtf8FirstByte.2 (Or.inr ?_)
+    obtain ⟨c, hc⟩ := Option.isSome_iff_exists.1 h
+    refine ⟨?_, ?_⟩
+    · have := ByteArray.le_size_of_utf8DecodeChar?_eq_some hc
+      have := c.utf8Size_pos
+      simp only [lt_iff, byteIdx_endPos, gt_iff_lt, ← size_bytes]
+      omega
+    · rw [getUtf8Byte]
+      exact ByteArray.isUtf8FirstByte_of_isSome_utf8DecodeChar? h
+
+theorem _root_.ByteArray.IsValidUtf8.isUtf8FirstByte_getElem_zero {b : ByteArray}
+    (h : b.IsValidUtf8) (h₀ : 0 < b.size) : b[0].IsUtf8FirstByte := by
+  rcases h with ⟨m, rfl⟩
+  have : m ≠ [] := by
+    rintro rfl
+    simp at h₀
+  conv => congr; congr; rw [← List.cons_head_tail this, ← List.singleton_append, List.utf8Encode_append]
+  rw [ByteArray.getElem_append_left]
+  · exact List.isUtf8FirstByte_getElem_utf8Encode_singleton.2 rfl
+  · simp [List.utf8Encode_singleton, Char.utf8Size_pos]
+
+theorem isUtf8FirstByte_getUtf8Byte_zero {b : String} {h} : (b.getUtf8Byte 0 h).IsUtf8FirstByte :=
+  b.isValidUtf8.isUtf8FirstByte_getElem_zero _
+
+protected theorem Pos.le_trans {a b c : Pos} : a ≤ b → b ≤ c → a ≤ c := by
+  simpa [le_iff] using Nat.le_trans
+
+protected theorem Pos.lt_of_lt_of_le {a b c : Pos} : a < b → b ≤ c → a < c := by
+  simpa [le_iff, lt_iff] using Nat.lt_of_lt_of_le
+
+theorem Pos.isValidUtf8_extract_iff {s : String} (p₁ p₂ : Pos) (hle : p₁ ≤ p₂) (hle' : p₂ ≤ s.endPos) :
+    (s.bytes.extract p₁.byteIdx p₂.byteIdx).IsValidUtf8 ↔ p₁ = p₂ ∨ (p₁.IsValid s ∧ p₂.IsValid s) := by
+  have hle'' : p₂.byteIdx ≤ s.bytes.size := by simpa [le_iff] using hle'
+  refine ⟨fun h => Classical.or_iff_not_imp_left.2 (fun h' => ?_), ?_⟩
+  · have hlt : p₁ < p₂ := by
+      simp_all [le_iff, lt_iff, Pos.ext_iff]
+      omega
+    have h₁ : p₁.IsValid s := by
+      rw [isValid_iff_isUtf8FirstByte]
+      refine Or.inr ⟨Pos.lt_of_lt_of_le hlt hle', ?_⟩
+      have hlt' : 0 < p₂.byteIdx - p₁.byteIdx := by
+        simp [lt_iff] at hlt
+        omega
+      have := h.isUtf8FirstByte_getElem_zero
+      simp only [ByteArray.size_extract, Nat.min_eq_left hle'', hlt', ByteArray.getElem_extract, Nat.add_zero] at this
+      simp [getUtf8Byte, this trivial]
+    refine ⟨h₁, ⟨hle', ?_⟩⟩
+    rw [ByteArray.extract_eq_extract_append_extract p₁.byteIdx (by simp) hle]
+    exact h₁.isValidUtf8_extract_zero.append h
+  · refine fun h => h.elim (by rintro rfl; simp) (fun ⟨h₁, h₂⟩ => ?_)
+    let t : String := ⟨_, h₂.isValidUtf8_extract_zero⟩
+    have htb : t.bytes = s.bytes.extract 0 p₂.byteIdx := rfl
+    have ht : p₁.IsValid t := by
+      refine ⟨?_, ?_⟩
+      · simpa [le_iff, t, Nat.min_eq_left hle'', ← size_bytes]
+      · simpa [htb, ByteArray.extract_extract, Nat.min_eq_left (le_iff.1 hle)] using h₁.isValidUtf8_extract_zero
+    simpa [htb, ByteArray.extract_extract, Nat.zero_add, Nat.min_eq_left hle'', ← size_bytes]
+      using ht.isValidUtf8_extract_utf8ByteSize
+
+theorem Pos.isValid_iff_isValidUtf8_extract_zero {s : String} {p : Pos} :
+    p.IsValid s ↔ p ≤ s.endPos ∧ (s.bytes.extract 0 p.byteIdx).IsValidUtf8 :=
+  ⟨fun ⟨h₁, h₂⟩ => ⟨h₁, h₂⟩, fun ⟨h₁, h₂⟩ => ⟨h₁, h₂⟩⟩
+
+theorem Pos.isValid_iff_isValidUtf8_extract_utf8ByteSize {s : String} {p : Pos} :
+    p.IsValid s ↔ p ≤ s.endPos ∧ (s.bytes.extract p.byteIdx s.utf8ByteSize).IsValidUtf8 := by
+  refine ⟨fun h => ⟨h.le_endPos, h.isValidUtf8_extract_utf8ByteSize⟩, fun ⟨h₁, h₂⟩ => ?_⟩
+  rw [← byteIdx_endPos, isValidUtf8_extract_iff _ _ h₁ (by simp [le_iff])] at h₂
+  obtain (rfl|h₂) := h₂
+  · simp
+  · exact h₂.1
+
+/--
+A `ValidPos s` is a byte offset in `s` together with a proof that this position is at a UTF-8
+character boundary.
+-/
+@[ext]
+structure ValidPos (s : String) where
+  /-- The underlying byte offset of the `ValidPos`. -/
+  offset : Pos
+  /-- The proof that `offset` is valid for the string `s`. -/
+  isValid : offset.IsValid s
+deriving @[expose] DecidableEq
+
+/-- The start position of `s`, as an `s.ValidPos`. -/
+@[inline, expose]
+def startValidPos (s : String) : s.ValidPos where
+  offset := 0
+  isValid := by simp
+
+instance {s : String} : Inhabited s.ValidPos where
+  default := s.startValidPos
+
+@[simp]
+theorem offset_startValidPos {s : String} : s.startValidPos.offset = 0 := (rfl)
+
+/-- The past-the-end position of `s`, as an `s.ValidPos`. -/
+@[inline, expose]
+def endValidPos (s : String) : s.ValidPos where
+  offset := s.endPos
+  isValid := by simp
+
+theorem ValidPos.isValidUtf8_extract {s : String} (pos₁ pos₂ : s.ValidPos) :
+    (s.bytes.extract pos₁.offset.byteIdx pos₂.offset.byteIdx).IsValidUtf8 := by
+  by_cases h : pos₁.offset ≤ pos₂.offset
+  · exact (Pos.isValidUtf8_extract_iff _ _   h pos₂.isValid.le_endPos).2 (Or.inr ⟨pos₁.isValid, pos₂.isValid⟩)
+  · rw [ByteArray.extract_eq_empty_iff.2]
+    · exact ByteArray.isValidUtf8_empty
+    · rw [Nat.min_eq_left]
+      · rw [Pos.le_iff] at h
+        omega
+      · have := Pos.le_iff.1 pos₂.isValid.le_endPos
+        rwa [size_bytes, ← byteIdx_endPos]
+
+/--
+A region or slice of some underlying string.
+
+A substring contains an string together with the start and end byte positions of a region of
+interest. Actually extracting a substring requires copying and memory allocation, while many
+substrings of the same underlying string may exist with very little overhead, and they are more
+convenient than tracking the bounds by hand.
+
+`String.Slice` bundles proofs to ensure that the start and end positions always delineate a valid
+string. For this reason, it should be preferred over `Substring`.
+-/
+structure Slice where
+  /-- The underlying strings. -/
+  str : String
+  /-- The byte position of the start of the string slice. -/
+  startInclusive : str.ValidPos
+  /-- The byte position of the end of the string slice. -/
+  endExclusive : str.ValidPos
+  /-- The slice is not degenerate (but it may be empty). -/
+  startInclusive_le_endExclusive : startInclusive.offset ≤ endExclusive.offset
+
+instance : Inhabited Slice where
+  default := ⟨"", "".startValidPos, "".startValidPos, by simp [Pos.le_iff]⟩
+
+@[inline, expose] -- expose for the defeq `s.toSlice.str = s`.
+def toSlice (s : String) : Slice where
+  str := s
+  startInclusive := s.startValidPos
+  endExclusive := s.endValidPos
+  startInclusive_le_endExclusive := by simp [Pos.le_iff]
+
+/-- The number of bytes of the UTF-8 encoding of the string slice. -/
+@[expose]
+def Slice.utf8ByteSize (s : Slice) : Pos :=
+  s.endExclusive.offset - s.startInclusive.offset
+
+@[simp]
+theorem Slice.byteIdx_utf8ByteSize {s : Slice} :
+    s.utf8ByteSize.byteIdx = s.endExclusive.offset.byteIdx - s.startInclusive.offset.byteIdx := (rfl)
+
+/-- Criterion for validity of positions in string slices. -/
+structure Pos.IsValidForSlice (s : Slice) (p : Pos) : Prop where
+  le_utf8ByteSize : p ≤ s.utf8ByteSize
+  isValid_add : (s.startInclusive.offset + p).IsValid s.str
+
+/--
+Accesses the indicated byte in the UTF-8 encoding of a string slice.
+
+At runtime, this function is implemented by efficient, constant-time code.
+-/
+@[inline, expose]
+def Slice.getUtf8Byte (s : Slice) (p : Pos) (h : p < s.utf8ByteSize) : UInt8 :=
+  s.str.getUtf8Byte (s.startInclusive.offset + p) (by
+    have := s.endExclusive.isValid.le_endPos
+    simp only [Pos.lt_iff, byteIdx_utf8ByteSize, Pos.le_iff, byteIdx_endPos, Pos.byteIdx_add] at *
+    omega)
+
+/--
+Accesses the indicated byte in the UTF-8 encoding of the string slice, or panics if the position
+is out-of-bounds.
+-/
+@[expose]
+def Slice.getUtf8Byte! (s : Slice) (p : String.Pos) : UInt8 :=
+  if h : p < s.utf8ByteSize then
+    s.getUtf8Byte p h
+  else
+    panic! "String slice access is out of bounds."
+
+@[extern "lean_string_utf8_extract"]
+def ValidPos.extract {s : @& String} (b e : @& s.ValidPos) : String where
+  bytes := s.bytes.extract b.offset.byteIdx e.offset.byteIdx
+  isValidUtf8 := b.isValidUtf8_extract e
+
+/-- Creates a `String` from a `String.Slice` by copying the bytes. -/
+@[inline]
+def Slice.copy (s : Slice) : String :=
+  s.startInclusive.extract s.endExclusive
+
+theorem Slice.bytes_copy {s : Slice} :
+    s.copy.bytes = s.str.bytes.extract s.startInclusive.offset.byteIdx s.endExclusive.offset.byteIdx := (rfl)
+
+@[simp]
+theorem Slice.utf8ByteSize_copy {s : Slice} :
+    s.copy.utf8ByteSize = s.endExclusive.offset.byteIdx - s.startInclusive.offset.byteIdx:= by
+  simp [← size_bytes, bytes_copy]
+  rw [Nat.min_eq_left (by simpa [Pos.le_iff] using s.endExclusive.isValid.le_endPos)]
+
+@[simp]
+theorem Slice.endPos_copy {s : Slice} : s.copy.endPos = s.utf8ByteSize := by
+  simp [Pos.ext_iff]
+
+theorem Slice.getUtf8Byte_eq_getUtf8Byte_copy {s : Slice} {p : Pos} {h : p < s.utf8ByteSize} :
+    s.getUtf8Byte p h = s.copy.getUtf8Byte p (by simpa) := by
+  simp [getUtf8Byte, String.getUtf8Byte, bytes_copy, ByteArray.getElem_extract]
+
+theorem Slice.getUtf8Byte_copy {s : Slice} {p : Pos} {h} :
+    s.copy.getUtf8Byte p h = s.getUtf8Byte p (by simpa using h) := by
+  rw [getUtf8Byte_eq_getUtf8Byte_copy]
+
+theorem Slice.isUtf8FirstByte_utf8ByteAt_zero {s : Slice} {h} :
+    (s.getUtf8Byte 0 h).IsUtf8FirstByte := by
+  simpa [getUtf8Byte_eq_getUtf8Byte_copy] using s.copy.isUtf8FirstByte_getUtf8Byte_zero
+
+@[simp]
+theorem Pos.add_zero {p : Pos} : p + 0 = p := by
+  simp [Pos.ext_iff]
+
+@[simp]
+theorem Pos.isValid_copy_iff {s : Slice} {p : Pos} :
+    p.IsValid s.copy ↔ p.IsValidForSlice s := by
+  refine ⟨fun ⟨h₁, h₂⟩ => ⟨?_, ?_⟩, fun ⟨h₁, h₂⟩ => ⟨?_, ?_⟩⟩
+  · simpa using h₁
+  · have := s.startInclusive_le_endExclusive
+    simp_all only [Slice.endPos_copy, le_iff, Slice.byteIdx_utf8ByteSize]
+    rw [Slice.bytes_copy, ByteArray.extract_extract, Nat.add_zero, Nat.min_eq_left (by omega)] at h₂
+    rw [← byteIdx_add, Pos.isValidUtf8_extract_iff] at h₂
+    · rcases h₂ with (h₂|⟨-, h₂⟩)
+      · rw [← h₂]
+        exact s.startInclusive.isValid
+      · exact h₂
+    · simp [le_iff]
+    · have := s.endExclusive.isValid.le_endPos
+      simp_all [le_iff]
+      omega
+  · simpa using h₁
+  · have := s.startInclusive_le_endExclusive
+    simp_all only [le_iff, Slice.byteIdx_utf8ByteSize]
+    rw [Slice.bytes_copy, ByteArray.extract_extract, Nat.add_zero, Nat.min_eq_left (by omega)]
+    rw [← byteIdx_add, Pos.isValidUtf8_extract_iff]
+    · exact Or.inr ⟨s.startInclusive.isValid, h₂⟩
+    · simp [le_iff]
+    · have := s.endExclusive.isValid.le_endPos
+      simp_all [le_iff]
+      omega
+
+/--
+A `Slice.Pos s` is a byte offset in `s` together with a proof that this position is at a UTF-8
+character boundary.
+-/
+@[ext]
+structure Slice.Pos (s : Slice) where
+  /-- The underlying byte offset of the `Slice.Pos`. -/
+  offset : String.Pos
+  /-- The proof that `offset` is valid for the string slice `s`. -/
+  isValidForSlice : offset.IsValidForSlice s
+deriving @[expose] DecidableEq
+
+/-- The start position of `s`, as an `s.Pos`. -/
+@[inline, expose]
+def Slice.startPos (s : Slice) : s.Pos where
+  offset := 0
+  isValidForSlice := ⟨by simp [Pos.le_iff], by simpa using s.startInclusive.isValid⟩
+
+@[simp]
+theorem ByteString.Slice.offset_startPos {s : Slice} : s.startPos.offset = 0 := (rfl)
+
+instance {s : Slice} : Inhabited s.Pos where
+  default := s.startPos
+
+@[simp]
+theorem Slice.offset_startInclusive_add_utf8ByteSize {s : Slice} :
+    s.startInclusive.offset + s.utf8ByteSize = s.endExclusive.offset := by
+  have := s.startInclusive_le_endExclusive
+  simp_all [String.Pos.ext_iff, Pos.le_iff]
+
+/-- The past-the-end position of `s`, as an `s.Pos`. -/
+@[inline, expose]
+def Slice.endPos (s : Slice) : s.Pos where
+  offset := s.utf8ByteSize
+  isValidForSlice := ⟨by simp [Pos.le_iff], by simpa using s.endExclusive.isValid⟩
+
+@[simp]
+theorem ByteString.Slice.offset_endPos {s : Slice} : s.endPos.offset = s.utf8ByteSize := (rfl)
+
+theorem Pos.isValidForSlice_iff_isUtf8FirstByte {s : Slice} {p : Pos} :
+    p.IsValidForSlice s ↔ (p = s.utf8ByteSize ∨ (∃ (h : p < s.utf8ByteSize), (s.getUtf8Byte p h).IsUtf8FirstByte)) := by
+  simp [← isValid_copy_iff, isValid_iff_isUtf8FirstByte, Slice.getUtf8Byte_copy]
+
+/-- Efficiently checks whether a position is at a UTF-8 character boundary of the slice `s`. -/
+@[expose]
+def Pos.isValidForSlice (s : Slice) (p : Pos) : Bool :=
+  if h : p < s.utf8ByteSize then
+    (s.getUtf8Byte p h).IsUtf8FirstByte
+  else
+    p = s.utf8ByteSize
+
+@[simp]
+theorem Pos.isValidForSlice_eq_true_iff {s : Slice} {p : Pos} :
+    p.isValidForSlice s = true ↔ p.IsValidForSlice s := by
+  rw [isValidForSlice_iff_isUtf8FirstByte]
+  fun_cases isValidForSlice with
+  | case1 h =>
+    simp_all only [decide_eq_true_eq, exists_true_left, iff_or_self]
+    rintro rfl
+    simp [lt_iff] at h
+  | case2 => simp_all
+
+@[simp]
+theorem Pos.isValidForSlice_eq_false_iff {s : Slice} {p : Pos} :
+    p.isValidForSlice s = false ↔ ¬ p.IsValidForSlice s := by
+  rw [← Bool.not_eq_true, isValidForSlice_eq_true_iff]
+
+instance {s : Slice} {p : Pos} : Decidable (p.IsValidForSlice s) :=
+  decidable_of_iff _ Pos.isValidForSlice_eq_true_iff
+
+theorem Pos.isValidForSlice_iff_isSome_utf8DecodeChar?_copy {s : Slice} {p : Pos} :
+    p.IsValidForSlice s ↔ p = s.utf8ByteSize ∨ (s.copy.bytes.utf8DecodeChar? p.byteIdx).isSome := by
+  rw [← isValid_copy_iff, isValid_iff_isSome_utf8DecodeChar?, Slice.endPos_copy]
+
+theorem Slice.bytes_str_eq {s : Slice} :
+    s.str.bytes = s.str.bytes.extract 0 s.startInclusive.offset.byteIdx ++
+      s.copy.bytes ++ s.str.bytes.extract s.endExclusive.offset.byteIdx s.str.bytes.size := by
+  rw [bytes_copy, ← ByteArray.extract_eq_extract_append_extract, ← ByteArray.extract_eq_extract_append_extract,
+    ByteArray.extract_zero_size]
+  · simp
+  · simpa [Pos.le_iff] using s.endExclusive.isValid.le_endPos
+  · simp
+  · simpa [Pos.le_iff] using s.startInclusive_le_endExclusive
+
+theorem Pos.isValidForSlice_iff_isSome_utf8DecodeChar? {s : Slice} {p : Pos} :
+    p.IsValidForSlice s ↔ p = s.utf8ByteSize ∨ (p < s.utf8ByteSize ∧ (s.str.bytes.utf8DecodeChar? (s.startInclusive.offset.byteIdx + p.byteIdx)).isSome) := by
+  refine ⟨?_, ?_⟩
+  · rw [isValidForSlice_iff_isSome_utf8DecodeChar?_copy]
+    rintro (rfl|h)
+    · simp
+    · refine Or.inr ⟨?_, ?_⟩
+      · have := ByteArray.lt_size_of_isSome_utf8DecodeChar? h
+        simpa [Pos.lt_iff] using this
+      · rw [ByteArray.utf8DecodeChar?_eq_utf8DecodeChar?_extract] at h
+        rw [Slice.bytes_str_eq, ByteArray.append_assoc, ByteArray.utf8DecodeChar?_eq_utf8DecodeChar?_extract]
+        simp only [ByteArray.size_append, ByteArray.size_extract, Nat.sub_zero, Nat.le_refl,
+          Nat.min_eq_left]
+        have h' : s.startInclusive.offset.byteIdx ≤ s.str.bytes.size := by
+          simpa [le_iff] using s.startInclusive.isValid.le_endPos
+        rw [Nat.min_eq_left h', ByteArray.extract_append_size_add' (by simp [size_bytes ▸ h']),
+          ByteArray.extract_append, Nat.add_sub_cancel_left]
+        rw [ByteArray.extract_eq_extract_append_extract s.copy.bytes.size]
+        · rw [ByteArray.append_assoc]
+          apply ByteArray.isSome_utf8DecodeChar?_append h
+        · have := ByteArray.lt_size_of_isSome_utf8DecodeChar? h
+          simp only [size_bytes, Slice.utf8ByteSize_copy, ByteArray.size_extract, Nat.le_refl,
+            Nat.min_eq_left] at this
+          simp only [size_bytes, Slice.utf8ByteSize_copy, ge_iff_le]
+          omega
+        · simp
+  · rw [isValidForSlice_iff_isUtf8FirstByte]
+    rintro (rfl|⟨h₁, h₂⟩)
+    · simp
+    · exact Or.inr ⟨h₁, ByteArray.isUtf8FirstByte_of_isSome_utf8DecodeChar? h₂⟩
+
+/-- Returns the byte at a position in a slice that is not the end position. -/
+@[inline, expose]
+def Slice.Pos.byte {s : Slice} (pos : s.Pos) (h : pos ≠ s.endPos) : UInt8 :=
+  s.getUtf8Byte pos.offset (by
+    have := pos.isValidForSlice.le_utf8ByteSize
+    simp_all [Pos.ext_iff, String.Pos.ext_iff, Pos.le_iff, Pos.lt_iff]
+    omega)
+
+theorem Slice.Pos.isUtf8FirstByte_byte {s : Slice} {pos : s.Pos} {h : pos ≠ s.endPos} :
+    (pos.byte h).IsUtf8FirstByte :=
+  ((Pos.isValidForSlice_iff_isUtf8FirstByte.1 pos.isValidForSlice).elim (fun h' => (h (Pos.ext h')).elim) (·.2))
+
+/-- Given a valid position on a slice `s`, obtains the corresponding valid position on the
+underlying string `s.str`. -/
+@[inline]
+def Slice.Pos.str {s : Slice} (pos : s.Pos) : s.str.ValidPos where
+  offset := s.startInclusive.offset + pos.offset
+  isValid := pos.isValidForSlice.isValid_add
+
+@[simp]
+theorem Slice.Pos.offset_str {s : Slice} {pos : s.Pos} :
+    pos.str.offset = s.startInclusive.offset + pos.offset := (rfl)
+
+@[simp]
+theorem Slice.Pos.offset_str_le_offset_endExclusive {s : Slice} {pos : s.Pos} :
+    pos.str.offset ≤ s.endExclusive.offset := by
+  have := pos.isValidForSlice.le_utf8ByteSize
+  have := s.startInclusive_le_endExclusive
+  simp only [Pos.le_iff, byteIdx_utf8ByteSize, offset_str, Pos.byteIdx_add, ge_iff_le] at *
+  omega
+
+theorem Slice.Pos.offset_le_offset_str {s : Slice} {pos : s.Pos} :
+    pos.offset ≤ pos.str.offset := by
+  simp [String.Pos.le_iff]
+
+@[simp]
+theorem Slice.Pos.offset_le_offset_endExclusive {s : Slice} {pos : s.Pos} :
+    pos.offset ≤ s.endExclusive.offset :=
+  Pos.le_trans offset_le_offset_str offset_str_le_offset_endExclusive
+
+/-- Given a slice and a valid position within the slice, obtain a new slice on the same underlying
+string by replacing the start of the slice with the given position. -/
+@[inline, expose] -- for the defeq `(s.replaceStart pos).str = s.str`
+def Slice.replaceStart (s : Slice) (pos : s.Pos) : Slice where
+  str := s.str
+  startInclusive := pos.str
+  endExclusive := s.endExclusive
+  startInclusive_le_endExclusive := Pos.offset_str_le_offset_endExclusive
+
+@[simp]
+theorem Slice.str_replaceStart {s : Slice} {pos : s.Pos} :
+    (s.replaceStart pos).str = s.str := rfl
+
+@[simp]
+theorem Slice.startInclusive_replaceStart {s : Slice} {pos : s.Pos} :
+    (s.replaceStart pos).startInclusive = pos.str := rfl
+
+@[simp]
+theorem Slice.endExclusive_replaceStart {s : Slice} {pos : s.Pos} :
+    (s.replaceStart pos).endExclusive = s.endExclusive := rfl
+
+/-- Given a slice and a valid position within the slice, obtain a new slice on the same underlying
+string by replacing the end of the slice with the given position. -/
+@[inline, expose] -- for the defeq `(s.replaceEnd pos).str = s.str`
+def Slice.replaceEnd (s : Slice) (pos : s.Pos) : Slice where
+  str := s.str
+  startInclusive := s.startInclusive
+  endExclusive := pos.str
+  startInclusive_le_endExclusive := by simp [String.Pos.le_iff]
+
+@[simp]
+theorem Slice.str_replaceEnd {s : Slice} {pos : s.Pos} :
+    (s.replaceEnd pos).str = s.str := rfl
+
+@[simp]
+theorem Slice.startInclusive_replaceEnd {s : Slice} {pos : s.Pos} :
+    (s.replaceEnd pos).startInclusive = s.startInclusive := rfl
+
+@[simp]
+theorem Slice.endExclusive_replaceEnd {s : Slice} {pos : s.Pos} :
+    (s.replaceEnd pos).endExclusive = pos.str := rfl
+
+/-- Given a slice and two valid positions within the slice, obtain a new slice on the same underlying
+string formed by the new bounds. -/
+@[inline, expose] -- for the defeq `(s.replaceStartEnd newStart newEnd).str = s.str`
+def Slice.replaceStartEnd (s : Slice) (newStart newEnd : s.Pos)
+    (h : newStart.offset ≤ newEnd.offset) : Slice where
+  str := s.str
+  startInclusive := newStart.str
+  endExclusive := newEnd.str
+  startInclusive_le_endExclusive := by simpa [Pos.le_iff] using h
+
+@[simp]
+theorem Slice.str_replaceStartEnd {s : Slice} {newStart newEnd : s.Pos} {h} :
+    (s.replaceStartEnd newStart newEnd h).str = s.str := rfl
+
+@[simp]
+theorem Slice.startInclusive_replaceStartEnd {s : Slice} {newStart newEnd : s.Pos} {h} :
+    (s.replaceStartEnd newStart newEnd h).startInclusive = newStart.str := rfl
+
+@[simp]
+theorem Slice.endExclusive_replaceStartEnd {s : Slice} {newStart newEnd : s.Pos} {h} :
+    (s.replaceStartEnd newStart newEnd h).endExclusive = newEnd.str := rfl
+
+/-- Given a slice and two valid positions within the slice, obtain a new slice on the same underlying
+string formed by the new bounds, or panic if the given end is strictly less than the given start. -/
+def Slice.replaceStartEnd! (s : Slice) (newStart newEnd : s.Pos) : Slice :=
+  if h : newStart.offset ≤ newEnd.offset then
+    s.replaceStartEnd newStart newEnd h
+  else
+    panic! "Starting position must be less than or equal to end position."
+
+@[simp]
+theorem Slice.utf8ByteSize_replaceStart {s : Slice} {pos : s.Pos} :
+    (s.replaceStart pos).utf8ByteSize = s.utf8ByteSize - pos.offset := by
+  ext
+  simp
+  omega
+
+@[simp]
+theorem Slice.utf8ByteSize_replaceEnd {s : Slice} {pos : s.Pos} :
+    (s.replaceEnd pos).utf8ByteSize = pos.offset := by
+  ext
+  simp
+
+@[simp]
+theorem Slice.utf8ByteSize_replaceStartEnd {s : Slice} {newStart newEnd : s.Pos} {h} :
+    (s.replaceStartEnd newStart newEnd h).utf8ByteSize = newEnd.offset - newStart.offset := by
+  ext
+  simp only [byteIdx_utf8ByteSize, str_replaceStartEnd, endExclusive_replaceStartEnd,
+    Pos.offset_str, Pos.byteIdx_add, startInclusive_replaceStartEnd, Pos.byteIdx_sub]
+  omega
+
+theorem Pos.add_comm (a b : Pos) : a + b = b + a := by
+  ext
+  simpa using Nat.add_comm _ _
+
+theorem Pos.add_assoc (a b c : Pos) : a + b + c = a + (b + c) := by
+  ext
+  simpa using Nat.add_assoc _ _ _
+
+theorem Pos.isValidForSlice_replaceStart {s : Slice} {p : s.Pos} {off : Pos} :
+    off.IsValidForSlice (s.replaceStart p) ↔ (p.offset + off).IsValidForSlice s := by
+  refine ⟨fun ⟨h₁, h₂⟩ => ⟨?_, ?_⟩, fun ⟨h₁, h₂⟩ => ⟨?_, ?_⟩⟩
+  · have := p.isValidForSlice.le_utf8ByteSize
+    simp_all [le_iff]
+    omega
+  · simp only [Slice.str_replaceStart, Slice.startInclusive_replaceStart, Slice.Pos.offset_str] at h₂
+    rwa [← Pos.add_assoc]
+  · simp_all [Pos.le_iff]
+    omega
+  · simp only [Slice.str_replaceStart, Slice.startInclusive_replaceStart, Slice.Pos.offset_str]
+    rwa [Pos.add_assoc]
+
+theorem Pos.isValidForSlice_replaceEnd {s : Slice} {p : s.Pos} {off : Pos} :
+    off.IsValidForSlice (s.replaceEnd p) ↔ off ≤ p.offset ∧ off.IsValidForSlice s := by
+  refine ⟨fun ⟨h₁, h₂⟩ => ⟨?_, ?_, ?_⟩, fun ⟨h₁, ⟨h₂, h₃⟩⟩ => ⟨?_, ?_⟩⟩
+  · simpa using h₁
+  · simp only [Slice.utf8ByteSize_replaceEnd] at h₁
+    exact Pos.le_trans h₁ p.isValidForSlice.le_utf8ByteSize
+  · simpa using h₂
+  · simpa using h₁
+  · simpa using h₃
+
+@[extern "lean_string_utf8_get", expose]
+def decodeChar (s : @& String) (byteIdx : @& Nat) (h : (s.bytes.utf8DecodeChar? byteIdx).isSome) : Char :=
+  s.bytes.utf8DecodeChar byteIdx h
+
+/-- Obtains the character at the given position in the string. -/
+@[inline, expose]
+def Slice.Pos.get {s : Slice} (pos : s.Pos) (h : pos ≠ s.endPos) : Char :=
+  s.str.decodeChar (s.startInclusive.offset.byteIdx + pos.offset.byteIdx)
+    ((Pos.isValidForSlice_iff_isSome_utf8DecodeChar?.1 pos.isValidForSlice).elim (by simp_all [Pos.ext_iff]) (·.2))
+
+theorem Slice.Pos.get_eq_utf8DecodeChar {s : Slice} (pos : s.Pos) (h : pos ≠ s.endPos) :
+    pos.get h = s.str.bytes.utf8DecodeChar (s.startInclusive.offset.byteIdx + pos.offset.byteIdx)
+      ((Pos.isValidForSlice_iff_isSome_utf8DecodeChar?.1 pos.isValidForSlice).elim (by simp_all [Pos.ext_iff]) (·.2)) := (rfl)
+
+/-- Returns the byte at the given position in the string, or `none` if the position is the end
+position. -/
+@[expose]
+def Slice.Pos.get? {s : Slice} (pos : s.Pos) : Option Char :=
+  if h : pos = s.endPos then none else some (pos.get h)
+
+/-- Returns the byte at the given position in the string, or panicks if the position is the end
+position. -/
+@[expose]
+def Slice.Pos.get! {s : Slice} (pos : s.Pos) : Char :=
+  if h : pos = s.endPos then panic! "Cannot retrieve character at end position" else pos.get h
+
+@[simp]
+theorem startInclusive_toSlice {s : String} : s.toSlice.startInclusive = s.startValidPos := rfl
+
+@[simp]
+theorem endExclusive_toSlice {s : String} : s.toSlice.endExclusive = s.endValidPos := rfl
+
+@[simp]
+theorem str_toSlice {s : String} : s.toSlice.str = s := rfl
+
+@[simp]
+theorem offset_endValidPos {s : String} : s.endValidPos.offset = s.endPos := (rfl)
+
+@[simp]
+theorem copy_toSlice {s : String} : s.toSlice.copy = s := by
+  simp [← bytes_inj, Slice.bytes_copy, ← size_bytes]
+
+@[simp]
+theorem Pos.isValidForSlice_toSlice_iff {s : String} {p : Pos} :
+    p.IsValidForSlice s.toSlice ↔ p.IsValid s := by
+  rw [← isValid_copy_iff, copy_toSlice]
+
+theorem Pos.IsValid.toSlice {s : String} {p : Pos} (h : p.IsValid s) :
+    p.IsValidForSlice s.toSlice :=
+  isValidForSlice_toSlice_iff.2 h
+
+theorem Pos.IsValidForSlice.ofSlice {s : String} {p : Pos} (h : p.IsValidForSlice s.toSlice) :
+    p.IsValid s :=
+  isValidForSlice_toSlice_iff.1 h
+
+/-- Turns a valid position on the string `s` into a valid position on the slice `s.toSlice`. -/
+@[inline, expose]
+def ValidPos.toSlice {s : String} (pos : s.ValidPos) : s.toSlice.Pos where
+  offset := pos.offset
+  isValidForSlice := pos.isValid.toSlice
+
+@[simp]
+theorem ValidPos.offset_toSlice {s : String} {pos : s.ValidPos} : pos.toSlice.offset = pos.offset := (rfl)
+
+/-- Given a string `s`, turns a valid position on the slice `s.toSlice` into a valid position on the
+string `s`. -/
+@[inline, expose]
+def Slice.Pos.ofSlice {s : String} (pos : s.toSlice.Pos) : s.ValidPos where
+  offset := pos.offset
+  isValid := pos.isValidForSlice.ofSlice
+
+@[simp]
+theorem Slice.Pos.ofset_ofSlice {s : String} {pos : s.toSlice.Pos} : pos.ofSlice.offset = pos.offset := (rfl)
+
+@[simp]
+theorem utf8ByteSize_toSlice {s : String} : s.toSlice.utf8ByteSize = s.endPos := by
+  rw [← Slice.endPos_copy, copy_toSlice]
+
+@[simp]
+theorem endPos_toSlice {s : String} : s.toSlice.endPos = s.endValidPos.toSlice :=
+  Slice.Pos.ext (by simp)
+
+@[simp]
+theorem startPos_toSlice {s : String} : s.toSlice.startPos = s.startValidPos.toSlice :=
+  Slice.Pos.ext (by simp)
+
+@[simp]
+theorem ValidPos.ofSlice_toSlice {s : String} (pos : s.ValidPos) : pos.toSlice.ofSlice = pos :=
+  ValidPos.ext (by simp)
+
+@[simp]
+theorem Slice.Pos.toSlice_ofSlice {s : String} (pos : s.toSlice.Pos) : pos.ofSlice.toSlice = pos :=
+  Slice.Pos.ext (by simp)
+
+/--
+Returns the character at the position `pos` of a string, taking a proof that `p` is not the
+past-the-end position.
+
+This function is overridden with an efficient implementation in runtime code.
+
+Examples:
+* `("abc".pos ⟨1⟩ (by decide)).get (by decide) = 'b'`
+* `("L∃∀N".pos ⟨1⟩ (by decide)).get (by decide) = '∃'`
+-/
+@[inline, expose]
+def ValidPos.get {s : String} (pos : s.ValidPos) (h : pos ≠ s.endValidPos) : Char :=
+  pos.toSlice.get (ne_of_apply_ne Slice.Pos.ofSlice (by simp [h]))
+
+/--
+Returns the character at the position `pos` of a string, or `none` if the position is the
+past-the-end position.
+
+This function is overridden with an efficient implementation in runtime code.
+-/
+@[inline, expose]
+def ValidPos.get? {s : String} (pos : s.ValidPos) : Option Char :=
+  pos.toSlice.get?
+
+/--
+Returns the character at the position `pos` of a string, or panics if the position is the
+past-the-end position.
+
+This function is overridden with an efficient implementation in runtime code.
+-/
+@[inline, expose]
+def ValidPos.get! {s : String} (pos : s.ValidPos) : Char :=
+  pos.toSlice.get!
+
+/--
+Returns the byte at the position `pos` of a string.
+-/
+@[inline, expose]
+def ValidPos.byte {s : String} (pos : s.ValidPos) (h : pos ≠ s.endValidPos) : UInt8 :=
+  pos.toSlice.byte (ne_of_apply_ne Slice.Pos.ofSlice (by simp [h]))
+
+@[simp]
+theorem append_left_inj {s₁ s₂ : String} (t : String) :
+    s₁ ++ t = s₂ ++ t ↔ s₁ = s₂ := by
+  simp [← String.data_inj]
+
+theorem append_assoc {s₁ s₂ s₃ : String} : s₁ ++ s₂ ++ s₃ = s₁ ++ (s₂ ++ s₃) := by
+  simp [← String.data_inj]
+
+@[simp]
+theorem utf8ByteSize_eq_zero_iff {s : String} : s.utf8ByteSize = 0 ↔ s = "" := by
+  refine ⟨fun h => ?_, fun h => h ▸ utf8ByteSize_empty⟩
+  simpa [← bytes_inj, ← ByteArray.size_eq_zero_iff] using h
+
+@[simp]
+theorem Pos.eq_zero_iff {p : Pos} : p = 0 ↔ p.byteIdx = 0 :=
+  Pos.ext_iff
+
+theorem endPos_eq_zero_iff {b : String} : b.endPos = 0 ↔ b = "" := by
+  simp
+
+@[simp]
+theorem startValidPos_eq_endValidPos_iff {b : String} : b.startValidPos = b.endValidPos ↔ b = "" := by
+  simp [← utf8ByteSize_eq_zero_iff, ValidPos.ext_iff, Eq.comm (b := b.endPos)]
+
+@[simp]
+theorem data_eq_nil_iff {b : String} : b.data = [] ↔ b = "" := by
+  rw [← List.asString_inj, asString_data, List.asString_nil]
+
+@[simp]
+theorem _root_.List.asString_eq_empty_iff {l : List Char} : l.asString = "" ↔ l = [] := by
+  rw [← data_inj, List.data_asString, data_empty]
+
+@[simp]
+theorem _root_.List.length_asString {l : List Char} : l.asString.length = l.length := by
+  rw [← String.length_data, List.data_asString]
+
+theorem isSome_utf8DecodeChar?_zero {b : String} (hb : b ≠ "") : (b.bytes.utf8DecodeChar? 0).isSome := by
+  refine (((Pos.isValid_iff_isSome_utf8DecodeChar? (s := b)).1 Pos.isValid_zero).elim ?_ id)
+  rw [eq_comm, endPos_eq_zero_iff]
+  exact fun h => (hb h).elim
+
+theorem head_data {b : String} {h} :
+    b.data.head h = b.bytes.utf8DecodeChar 0 (isSome_utf8DecodeChar?_zero (by simpa using h)) := by
+  obtain ⟨l, rfl⟩ := b.exists_eq_asString
+  match l with
+  | [] => simp at h
+  | c::cs => simp
+
+theorem get_startValidPos {b : String} (h) :
+    b.startValidPos.get h = b.data.head (by rwa [ne_eq, data_eq_nil_iff, ← startValidPos_eq_endValidPos_iff]) :=
+  head_data.symm
+
+theorem eq_singleton_append {s : String} (h : s.startValidPos ≠ s.endValidPos) :
+    ∃ t, s = singleton (s.startValidPos.get h) ++ t := by
+  obtain ⟨m, rfl⟩ := s.exists_eq_asString
+  have hm : m ≠ [] := by
+    rwa [ne_eq, ← List.asString_eq_empty_iff, ← startValidPos_eq_endValidPos_iff]
+  refine ⟨m.tail.asString, ?_⟩
+  rw (occs := [1]) [← List.cons_head_tail hm]
+  rw [← List.singleton_append, List.asString_append, append_left_inj, ← singleton_eq_asString,
+    get_startValidPos]
+  simp
+
+theorem Slice.copy_eq_copy_replaceEnd {s : Slice} {pos : s.Pos} :
+    s.copy = (s.replaceEnd pos).copy ++ (s.replaceStart pos).copy := by
+  rw [← String.bytes_inj, bytes_copy, bytes_append, bytes_copy, bytes_copy]
+  simp only [str_replaceEnd, startInclusive_replaceEnd, endExclusive_replaceEnd,
+    Slice.Pos.offset_str, Pos.byteIdx_add, str_replaceStart, startInclusive_replaceStart,
+    endExclusive_replaceStart, ByteArray.extract_append_extract, Nat.le_add_right, Nat.min_eq_left]
+  rw [Nat.max_eq_right]
+  exact pos.offset_str_le_offset_endExclusive
+
+/-- Given a slice `s` and a position on `s.copy`, obtain the corresponding position on `s`. -/
+@[inline]
+def ValidPos.ofCopy {s : Slice} (pos : s.copy.ValidPos) : s.Pos where
+  offset := pos.offset
+  isValidForSlice := Pos.isValid_copy_iff.1 pos.isValid
+
+@[simp]
+theorem ValidPos.offset_ofCopy {s : Slice} {pos : s.copy.ValidPos} : pos.ofCopy.offset = pos.offset := (rfl)
+
+/-- Given a slice `s` and a position on `s`, obtain the corresponding position on `s.copy.` -/
+@[inline]
+def Slice.Pos.toCopy {s : Slice} (pos : s.Pos) : s.copy.ValidPos where
+  offset := pos.offset
+  isValid := Pos.isValid_copy_iff.2 pos.isValidForSlice
+
+@[simp]
+theorem Slice.Pos.offset_toCopy {s : Slice} {pos : s.Pos} : pos.toCopy.offset = pos.offset := (rfl)
+
+@[simp]
+theorem Slice.Pos.ofCopy_toCopy {s : Slice} {pos : s.Pos} : pos.toCopy.ofCopy = pos :=
+  Slice.Pos.ext (by simp)
+
+@[simp]
+theorem ValidPos.toCopy_ofCopy {s : Slice} {pos : s.copy.ValidPos} : pos.ofCopy.toCopy = pos :=
+  ValidPos.ext (by simp)
+
+theorem ValidPos.ofCopy_inj {s : Slice} {pos pos' : s.copy.ValidPos} : pos.ofCopy = pos'.ofCopy ↔ pos = pos' :=
+  ⟨fun h => by simpa using congrArg Slice.Pos.toCopy h, (· ▸ rfl)⟩
+
+@[simp]
+theorem Slice.startValidPos_copy {s : Slice} : s.copy.startValidPos = s.startPos.toCopy :=
+  ValidPos.ext (by simp)
+
+@[simp]
+theorem Slice.endValidPos_copy {s : Slice} : s.copy.endValidPos = s.endPos.toCopy :=
+  ValidPos.ext (by simp)
+
+theorem Slice.Pos.get_toCopy {s : Slice} {pos : s.Pos} (h) :
+    pos.toCopy.get h = pos.get (by rintro rfl; simp at h) := by
+  rw [ValidPos.get, Slice.Pos.get_eq_utf8DecodeChar, Slice.Pos.get_eq_utf8DecodeChar]
+  simp only [str_toSlice, bytes_copy, startInclusive_toSlice, startValidPos_copy, offset_toCopy,
+    ByteString.Slice.offset_startPos, Pos.byteIdx_zero, ValidPos.offset_toSlice, Nat.zero_add]
+  rw [ByteArray.utf8DecodeChar_eq_utf8DecodeChar_extract]
+  conv => lhs; congr; rw [ByteArray.extract_extract]
+  conv => rhs; rw [ByteArray.utf8DecodeChar_eq_utf8DecodeChar_extract]
+  exact ByteArray.utf8DecodeChar_extract_congr _ _ _
+
+theorem Slice.Pos.get_eq_get_toCopy {s : Slice} {pos : s.Pos} {h} :
+    pos.get h = pos.toCopy.get (ne_of_apply_ne ValidPos.ofCopy (by simp [h])) :=
+  (get_toCopy _).symm
+
+theorem Slice.Pos.byte_toCopy {s : Slice} {pos : s.Pos} (h) :
+    pos.toCopy.byte h = pos.byte (by rintro rfl; simp at h) := by
+  rw [ValidPos.byte, Slice.Pos.byte, Slice.Pos.byte]
+  simp [getUtf8Byte, String.getUtf8Byte, bytes_copy, ByteArray.getElem_extract]
+
+theorem Slice.Pos.byte_eq_byte_toCopy {s : Slice} {pos : s.Pos} {h} :
+    pos.byte h = pos.toCopy.byte (ne_of_apply_ne ValidPos.ofCopy (by simp [h])) :=
+  (byte_toCopy _).symm
+
+/-- Given a position in `s.replaceStart p₀`, obtain the corresponding position in `s`. -/
+@[inline]
+def Slice.Pos.ofReplaceStart {s : Slice} {p₀ : s.Pos} (pos : (s.replaceStart p₀).Pos) : s.Pos where
+  offset := p₀.offset + pos.offset
+  isValidForSlice := Pos.isValidForSlice_replaceStart.1 pos.isValidForSlice
+
+@[simp]
+theorem Slice.Pos.offset_ofReplaceStart {s : Slice} {p₀ : s.Pos} {pos : (s.replaceStart p₀).Pos} :
+    (ofReplaceStart pos).offset = p₀.offset + pos.offset := (rfl)
+
+/-- Given a position in `s` that is at least `p₀`, obtain the corresponding position in
+`s.replaceStart p₀`. -/
+@[inline]
+def Slice.Pos.toReplaceStart {s : Slice} (p₀ : s.Pos) (pos : s.Pos) (h : p₀.offset ≤ pos.offset) :
+    (s.replaceStart p₀).Pos where
+  offset := pos.offset - p₀.offset
+  isValidForSlice := Pos.isValidForSlice_replaceStart.2 (by
+    have : p₀.offset + (pos.offset - p₀.offset) = pos.offset := by
+      simp_all [Pos.le_iff, String.Pos.ext_iff]
+    simpa [this] using pos.isValidForSlice)
+
+@[simp]
+theorem Slice.Pos.offset_toReplaceStart {s : Slice} {p₀ : s.Pos} {pos : s.Pos} {h} :
+    (toReplaceStart p₀ pos h).offset = pos.offset - p₀.offset := (rfl)
+
+@[simp]
+theorem Slice.Pos.ofReplaceStart_startPos {s : Slice} {pos : s.Pos} :
+    ofReplaceStart (s.replaceStart pos).startPos = pos :=
+  Slice.Pos.ext (by simp)
+
+@[simp]
+theorem Slice.Pos.ofReplaceStart_endPos {s : Slice} {pos : s.Pos} :
+    ofReplaceStart (s.replaceStart pos).endPos = s.endPos := by
+  have := pos.isValidForSlice.le_utf8ByteSize
+  simp_all [Pos.ext_iff, String.Pos.ext_iff, Pos.le_iff]
+
+theorem Slice.Pos.ofReplaceStart_inj {s : Slice} {p₀ : s.Pos} {pos pos' : (s.replaceStart p₀).Pos} :
+    ofReplaceStart pos = ofReplaceStart pos' ↔ pos = pos' := by
+  simp [Pos.ext_iff, String.Pos.ext_iff]
+
+theorem Slice.Pos.get_eq_get_ofReplaceStart {s : Slice} {p₀ : s.Pos} {pos : (s.replaceStart p₀).Pos} {h} :
+    pos.get h = (ofReplaceStart pos).get (by rwa [← ofReplaceStart_endPos, ne_eq, ofReplaceStart_inj]) := by
+  simp [Slice.Pos.get, Nat.add_assoc]
+
+theorem Slice.Pos.copy_eq_append_get {s : Slice} {pos : s.Pos} (h : pos ≠ s.endPos) :
+    ∃ t₁ t₂ : String, s.copy = t₁ ++ singleton (pos.get h) ++ t₂ ∧ t₁.utf8ByteSize = pos.offset.byteIdx := by
+  obtain ⟨t₂, ht₂⟩ := (s.replaceStart pos).copy.eq_singleton_append (by simpa [← ValidPos.ofCopy_inj, ← ofReplaceStart_inj])
+  refine ⟨(s.replaceEnd pos).copy, t₂, ?_, by simp⟩
+  simp only [Slice.startValidPos_copy, get_toCopy, get_eq_get_ofReplaceStart, ofReplaceStart_startPos] at ht₂
+  rw [append_assoc, ← ht₂, ← copy_eq_copy_replaceEnd]
+
+theorem Slice.Pos.utf8ByteSize_byte {s : Slice} {pos : s.Pos} {h : pos ≠ s.endPos} :
+    (pos.byte h).utf8ByteSize pos.isUtf8FirstByte_byte = ⟨(pos.get h).utf8Size⟩ := by
+  simp [getUtf8Byte, byte, String.getUtf8Byte, get_eq_utf8DecodeChar, ByteArray.utf8Size_utf8DecodeChar]
+
+/-- Advances a valid position on a slice to the next valid position, given a proof that the
+position is not the past-the-end position, which guarantees that such a position exists. -/
+@[expose]
+def Slice.Pos.next {s : Slice} (pos : s.Pos) (h : pos ≠ s.endPos) : s.Pos where
+  offset := pos.offset + (pos.byte h).utf8ByteSize pos.isUtf8FirstByte_byte
+  isValidForSlice := by
+    obtain ⟨t₁, t₂, ht, ht'⟩ := copy_eq_append_get h
+    replace ht' : pos.offset = ⟨t₁.utf8ByteSize⟩ := Eq.symm (String.Pos.ext ht')
+    rw [utf8ByteSize_byte, ← Pos.isValid_copy_iff, ht, ht']
+    refine Pos.IsValid.append_right ?_ t₂
+    refine Pos.IsValid.append_left ?_ t₁
+    exact Pos.isValid_singleton.2 (Or.inr rfl)
+
+/-- Advances a valid position on a slice to the next valid position, or returns `none` if the
+given position is the past-the-end position. -/
+@[expose]
+def Slice.Pos.next? {s : Slice} (pos : s.Pos) : Option s.Pos :=
+  if h : pos = s.endPos then none else some (pos.next h)
+
+/-- Advances a valid position on a slice to the next valid position, or panics if the given
+position is the past-the-end position. -/
+@[expose]
+def Slice.Pos.next! {s : Slice} (pos : s.Pos) : s.Pos :=
+  if h : pos = s.endPos then panic! "Cannot advance the end position" else pos.next h
+
+@[simp]
+theorem Slice.Pos.byteIdx_offset_next {s : Slice} {pos : s.Pos} {h : pos ≠ s.endPos} :
+    (pos.next h).offset.byteIdx = pos.offset.byteIdx + (pos.get h).utf8Size := by
+  simp [next, utf8ByteSize_byte]
+
+/-- Increases the byte offset of the position by `1`. Not to be confused with `ValidPos.next`. -/
+@[inline, expose]
+def Pos.inc (p : Pos) : Pos :=
+  ⟨p.byteIdx + 1⟩
+
+@[simp]
+theorem Pos.byteIdx_inc {p : Pos} : p.inc.byteIdx = p.byteIdx + 1 := (rfl)
+
+/-- Decreases the byte offset of the position by `1`. Not to be confused with `ValidPos.prev`. -/
+@[inline, expose]
+def Pos.dec (p : Pos) : Pos :=
+  ⟨p.byteIdx - 1⟩
+
+@[simp]
+theorem Pos.byteIdx_dec {p : Pos} : p.dec.byteIdx = p.byteIdx - 1 := (rfl)
+
+@[inline, expose]
+def Slice.Pos.prevAux {s : Slice} (pos : s.Pos) (h : pos ≠ s.startPos) : String.Pos :=
+  go (pos.offset.byteIdx - 1) (by
+    have := pos.isValidForSlice.le_utf8ByteSize
+    simp [Pos.le_iff, Pos.lt_iff, Pos.ext_iff] at ⊢ this h
+    omega)
+where
+  go (off : Nat) (h₁ : ⟨off⟩ < s.utf8ByteSize) : String.Pos :=
+    if hbyte : (s.getUtf8Byte ⟨off⟩ h₁).IsUtf8FirstByte then
+      ⟨off⟩
+    else
+      have : 0 ≠ off := by
+        intro h
+        obtain hoff : (⟨off⟩ : String.Pos) = 0 := by simpa [String.Pos.ext_iff] using h.symm
+        simp [hoff, s.isUtf8FirstByte_utf8ByteAt_zero] at hbyte
+      match off with
+      | 0 => False.elim (by contradiction)
+      | off + 1 => go off (by simp [Pos.lt_iff] at ⊢ h₁; omega)
+  termination_by structural off
+
+theorem Pos.isValidForSlice_prevAuxGo {s : Slice} (off : Nat) (h₁ : ⟨off⟩ < s.utf8ByteSize) :
+    (Slice.Pos.prevAux.go off h₁).IsValidForSlice s := by
+  induction off with
+  | zero =>
+    rw [Slice.Pos.prevAux.go]
+    split
+    · exact Pos.isValidForSlice_iff_isUtf8FirstByte.2 (Or.inr ⟨_, ‹_›⟩)
+    · simpa using elim
+  | succ off ih =>
+    rw [Slice.Pos.prevAux.go]
+    split
+    · exact Pos.isValidForSlice_iff_isUtf8FirstByte.2 (Or.inr ⟨_, ‹_›⟩)
+    · simpa using ih _
+where
+  elim {P : Pos → Prop} {h : False} : P h.elim := h.elim
+
+theorem Pos.isValidForSlice_prevAux {s : Slice} (pos : s.Pos) (h : pos ≠ s.startPos) :
+    (pos.prevAux h).IsValidForSlice s :=
+  isValidForSlice_prevAuxGo ..
+
+/-- Returns the previous valid position before the given position, given a proof that the position
+is not the start position, which guarantees that such a position exists. -/
+@[inline, expose]
+def Slice.Pos.prev {s : Slice} (pos : s.Pos) (h : pos ≠ s.startPos) : s.Pos where
+  offset := prevAux pos h
+  isValidForSlice := Pos.isValidForSlice_prevAux _ _
+
+/-- Returns the previous valid position before the given position, or `none` if the position is
+the start position. -/
+@[expose]
+def Slice.Pos.prev? {s : Slice} (pos : s.Pos) : Option s.Pos :=
+  if h : pos = s.startPos then none else some (pos.prev h)
+
+/-- Returns the previous valid position before the given position, or panics if the position is
+the start position. -/
+@[expose]
+def Slice.Pos.prev! {s : Slice} (pos : s.Pos) : s.Pos :=
+  if h : pos = s.startPos then panic! "The start position has no previous position" else pos.prev h
+
+/-- Constructs a valid position on `s` from a position and a proof that it is valid. -/
+@[inline, expose]
+def Slice.pos (s : Slice) (off : String.Pos) (h : off.IsValidForSlice s) : s.Pos where
+  offset := off
+  isValidForSlice := h
+
+@[simp]
+theorem Slice.offset_pos {s : Slice} {off h} : (s.pos off h).offset = off := rfl
+
+/-- Constructs a valid position on `s` from a position, returning `none` if the position is not valid. -/
+@[expose]
+def Slice.pos? (s : Slice) (off : String.Pos) : Option s.Pos :=
+  if h : off.isValidForSlice s then
+    some (s.pos off (Pos.isValidForSlice_eq_true_iff.1 h))
+  else
+    none
+
+/-- Constructs a valid position `s` from a position, panicking if the position is not valid. -/
+@[expose]
+def Slice.pos! (s : Slice) (off : String.Pos) : s.Pos :=
+  if h : off.isValidForSlice s then
+    s.pos off (Pos.isValidForSlice_eq_true_iff.1 h)
+  else
+    panic! "Offset is not at a valid UTF-8 character boundary"
+
+/-- Advances a valid position on a string to the next valid position, given a proof that the
+position is not the past-the-end position, which guarantees that such a position exists. -/
+@[inline, expose]
+def ValidPos.next {s : String} (pos : s.ValidPos) (h : pos ≠ s.endValidPos) : s.ValidPos :=
+  (pos.toSlice.next (ne_of_apply_ne Slice.Pos.ofSlice (by simpa))).ofSlice
+
+/-- Advances a valid position on a string to the next valid position, or returns `none` if the
+given position is the past-the-end position. -/
+@[inline, expose]
+def ValidPos.next? {s : String} (pos : s.ValidPos) : Option s.ValidPos :=
+  pos.toSlice.next?.map Slice.Pos.ofSlice
+
+/-- Advances a valid position on a string to the next valid position, or panics if the given
+position is the past-the-end position. -/
+@[inline, expose]
+def ValidPos.next! {s : String} (pos : s.ValidPos) : s.ValidPos :=
+  pos.toSlice.next!.ofSlice
+
+/-- Returns the previous valid position before the given position, given a proof that the position
+is not the start position, which guarantees that such a position exists. -/
+@[inline, expose]
+def ValidPos.prev {s : String} (pos : s.ValidPos) (h : pos ≠ s.startValidPos) : s.ValidPos :=
+  (pos.toSlice.prev (ne_of_apply_ne Slice.Pos.ofSlice (by simpa))).ofSlice
+
+/-- Returns the previous valid position before the given position, or `none` if the position is
+the start position. -/
+@[inline, expose]
+def ValidPos.prev? {s : String} (pos : s.ValidPos) : Option s.ValidPos :=
+  pos.toSlice.prev?.map Slice.Pos.ofSlice
+
+/-- Returns the previous valid position before the given position, or panics if the position is
+the start position. -/
+@[inline, expose]
+def ValidPos.prev! {s : String} (pos : s.ValidPos) : s.ValidPos :=
+  pos.toSlice.prev!.ofSlice
+
+/-- Constructs a valid position on `s` from a position and a proof that it is valid. -/
+@[inline, expose]
+def pos (s : String) (off : Pos) (h : off.IsValid s) : s.ValidPos :=
+  (s.toSlice.pos off h.toSlice).ofSlice
+
+/-- Constructs a valid position on `s` from a position, returning `none` if the position is not valid. -/
+@[inline, expose]
+def pos? (s : String) (off : Pos) : Option s.ValidPos :=
+  (s.toSlice.pos? off).map Slice.Pos.ofSlice
+
+/-- Constructs a valid position `s` from a position, panicking if the position is not valid. -/
+@[inline, expose]
+def pos! (s : String) (off : Pos) : s.ValidPos :=
+  (s.toSlice.pos! off).ofSlice
+
+/-- Constructs a valid position on `t` from a valid position on `s` and a proof that `s = t`. -/
+@[inline]
+def Slice.Pos.cast {s t : Slice} (pos : s.Pos) (h : s = t) : t.Pos where
+  offset := pos.offset
+  isValidForSlice := h ▸ pos.isValidForSlice
+
+@[simp]
+theorem Slice.Pos.offset_cast {s t : Slice} {pos : s.Pos} {h : s = t} :
+    (pos.cast h).offset = pos.offset := (rfl)
+
+@[simp]
+theorem Slice.Pos.cast_rfl {s : Slice} {pos : s.Pos} : pos.cast rfl = pos :=
+  Slice.Pos.ext (by simp)
+
+/-- Constructs a valid position on `t` from a valid position on `s` and a proof that `s = t`. -/
+@[inline]
+def ValidPos.cast {s t : String} (pos : s.ValidPos) (h : s = t) : t.ValidPos where
+  offset := pos.offset
+  isValid := h ▸ pos.isValid
+
+@[simp]
+theorem ValidPos.offset_cast {s t : String} {pos : s.ValidPos} {h : s = t} :
+    (pos.cast h).offset = pos.offset := (rfl)
+
+@[simp]
+theorem ValidPos.cast_rfl {s : String} {pos : s.ValidPos} : pos.cast rfl = pos :=
+  ValidPos.ext (by simp)
+
+/-- Given a byte position within a string slice, obtains the smallest valid position that is
+strictly greater than the given byte position. -/
+@[inline]
+def Slice.findNextPos (offset : String.Pos) (s : Slice) (_h : offset < s.utf8ByteSize) : s.Pos :=
+  go offset.inc
+where
+  go (offset : String.Pos) : s.Pos :=
+    if h : offset < s.utf8ByteSize then
+      if h' : (s.getUtf8Byte offset h).IsUtf8FirstByte then
+        s.pos offset (Pos.isValidForSlice_iff_isUtf8FirstByte.2 (Or.inr ⟨_, h'⟩))
+      else
+        go offset.inc
+    else
+      s.endPos
+  termination_by s.utf8ByteSize.byteIdx - offset.byteIdx
+  decreasing_by
+    simp only [Pos.lt_iff, byteIdx_utf8ByteSize, Pos.byteIdx_inc, gt_iff_lt] at h ⊢
+    omega
+
+@[simp]
+theorem Pos.le_refl {p : Pos} : p ≤ p := by simp [le_iff]
+
+theorem Pos.lt_inc {p : Pos} : p < p.inc := by simp [lt_iff]
+
+theorem Pos.le_of_lt {p q : Pos} : p < q → p ≤ q := by simpa [lt_iff, le_iff] using Nat.le_of_lt
+
+theorem Pos.inc_le {p q : Pos} : p.inc ≤ q ↔ p < q := by simpa [lt_iff, le_iff] using Nat.succ_le
+
+private theorem Slice.le_offset_findNextPosGo {s : Slice} {o : String.Pos} (h : o ≤ s.utf8ByteSize) :
+    o ≤ (findNextPos.go s o).offset := by
+  fun_induction findNextPos.go with
+  | case1 => simp
+  | case2 x h₁ h₂ ih =>
+    refine Pos.le_of_lt (Pos.lt_of_lt_of_le Pos.lt_inc (ih ?_))
+    rw [Pos.le_iff, Pos.byteIdx_inc]
+    exact Nat.succ_le.2 h₁
+  | case3 x h => exact h
+
+theorem Slice.lt_offset_findNextPos {s : Slice} {o : String.Pos} (h) : o < (s.findNextPos o h).offset :=
+  Pos.lt_of_lt_of_le Pos.lt_inc (le_offset_findNextPosGo (Pos.inc_le.2 h))
+
+theorem Slice.Pos.prevAuxGo_le_self {s : Slice} {p : Nat} {h : ⟨p⟩ < s.utf8ByteSize} :
+    prevAux.go p h ≤ ⟨p⟩ := by
+  induction p with
+  | zero =>
+    rw [prevAux.go]
+    split
+    · simp
+    · simpa using elim (· ≤ { })
+  | succ p ih =>
+    rw [prevAux.go]
+    split
+    · simp
+    · simpa using Nat.le_trans ih (by simp)
+where
+  elim (P : String.Pos → Prop) {h : False} : P h.elim := h.elim
+
+theorem Pos.lt_of_le_of_lt {a b c : Pos} : a ≤ b → b < c → a < c := by
+  simpa [le_iff, lt_iff] using Nat.lt_of_le_of_lt
+
+theorem Slice.Pos.prevAux_lt_self {s : Slice} {p : s.Pos} {h} : p.prevAux h < p.offset := by
+  rw [prevAux]
+  refine Pos.lt_of_le_of_lt prevAuxGo_le_self ?_
+  simp [Pos.ext_iff, Pos.lt_iff] at *
+  omega
+
+theorem Slice.Pos.prevAux_lt_utf8ByteSize {s : Slice} {p : s.Pos} {h} : p.prevAux h < s.utf8ByteSize :=
+  Pos.lt_of_lt_of_le prevAux_lt_self p.isValidForSlice.le_utf8ByteSize
+
+theorem Pos.ne_of_lt {a b : Pos} : a < b → a ≠ b := by
+  simpa [lt_iff, Pos.ext_iff] using Nat.ne_of_lt
+
+theorem Slice.Pos.prev_ne_endPos {s : Slice} {p : s.Pos} {h} : p.prev h ≠ s.endPos := by
+  simpa [Pos.ext_iff, prev] using Pos.ne_of_lt prevAux_lt_utf8ByteSize
+
+theorem Slice.Pos.offset_prev_lt_offset {s : Slice} {p : s.Pos} {h} : (p.prev h).offset < p.offset := by
+  simpa [prev] using prevAux_lt_self
+
+/-- Advances the position `p` `n` times, saturating at `s.endPos` if necessary. -/
+def Slice.Pos.nextn {s : Slice} (p : s.Pos) (n : Nat) : s.Pos :=
+  match n with
+  | 0 => p
+  | n + 1 =>
+    if h : p ≠ s.endPos then
+      nextn (p.next h) n
+    else
+      p
+
+/-- Iterates `p.prev` `n` times, saturating at `s.startPos` if necessary. -/
+def Slice.Pos.prevn {s : Slice} (p : s.Pos) (n : Nat) : s.Pos :=
+  match n with
+  | 0 => p
+  | n + 1 =>
+    if h : p ≠ s.startPos then
+      prevn (p.prev h) n
+    else
+      p
+
+@[expose]
 def utf8GetAux : List Char → Pos → Pos → Char
   | [],    _, _ => default
   | c::cs, i, p => if i = p then c else utf8GetAux cs (i + c) p
@@ -486,6 +1975,7 @@ Examples:
 def get (s : @& String) (p : @& Pos) : Char :=
   utf8GetAux s.data 0 p
 
+@[expose]
 def utf8GetAux? : List Char → Pos → Pos → Option Char
   | [],    _, _ => none
   | c::cs, i, p => if i = p then some c else utf8GetAux? cs (i + c) p
@@ -503,7 +1993,7 @@ Examples:
 * `"L∃∀N".get? ⟨1⟩ = some '∃'`
 * `"L∃∀N".get? ⟨2⟩ = none`
 -/
-@[extern "lean_string_utf8_get_opt"]
+@[extern "lean_string_utf8_get_opt", expose]
 def get? : (@& String) → (@& Pos) → Option Char
   | s, p => utf8GetAux? s.data 0 p
 
@@ -523,6 +2013,7 @@ def get! (s : @& String) (p : @& Pos) : Char :=
   match s with
   | s => utf8GetAux s.data 0 p
 
+@[expose]
 def utf8SetAux (c' : Char) : List Char → Pos → Pos → List Char
   | [],    _, _ => []
   | c::cs, i, p =>
@@ -542,7 +2033,7 @@ Examples:
 * `"L∃∀N".set ⟨2⟩ 'X' = "L∃∀N"` because `'∃'` is a multi-byte character, so the byte index `2` is an
   invalid position.
 -/
-@[extern "lean_string_utf8_set"]
+@[extern "lean_string_utf8_set", expose]
 def set : String → (@& Pos) → Char → String
   | s, i, c => (utf8SetAux c s.data 0 i).asString
 
@@ -557,6 +2048,7 @@ Examples:
 * `"abc".modify ⟨1⟩ Char.toUpper = "aBc"`
 * `"abc".modify ⟨3⟩ Char.toUpper = "abc"`
 -/
+@[expose]
 def modify (s : String) (i : Pos) (f : Char → Char) : String :=
   s.set i <| f <| s.get i
 
@@ -580,6 +2072,7 @@ def next (s : @& String) (p : @& Pos) : Pos :=
   let c := get s p
   p + c
 
+@[expose]
 def utf8PrevAux : List Char → Pos → Pos → Pos
   | [],    _, p => ⟨p.byteIdx - 1⟩
   | c::cs, i, p =>
@@ -609,7 +2102,7 @@ Examples:
 * `"abc".front = 'a'`
 * `"".front = (default : Char)`
 -/
-@[inline] def front (s : String) : Char :=
+@[inline, expose] def front (s : String) : Char :=
   get s 0
 
 @[export lean_string_front]
@@ -623,7 +2116,7 @@ Examples:
 * `"abc".back = 'c'`
 * `"".back = (default : Char)`
 -/
-@[inline] def back (s : String) : Char :=
+@[inline, expose] def back (s : String) : Char :=
   get s (prev s s.endPos)
 
 /--
@@ -864,7 +2357,6 @@ where
     | [],    _, _ => []
     | c::cs, i, e => if i = e then [] else c :: go₂ cs (i + c) e
 
-
 @[specialize] def splitAux (s : String) (p : Char → Bool) (b : Pos) (i : Pos) (r : List String) : List String :=
   if h : s.atEnd i then
     let r := (s.extract b i)::r
@@ -918,7 +2410,6 @@ def splitOnAux (s sep : String) (b : Pos) (i : Pos) (j : Pos) (r : List String) 
       splitOnAux s sep b (s.next (i - j)) 0 r
 termination_by (s.endPos.1 - (i - j).1, sep.endPos.1 - j.1)
 decreasing_by
-  all_goals simp_wf
   focus
     rename_i h _ _
     left; exact Nat.sub_lt_sub_left
@@ -1633,7 +3124,7 @@ string, then the character at the start position is returned. If the substring's
 not a valid position in the string, the fallback value `(default : Char)`, which is `'A'`, is
 returned.  Does not panic.
 -/
-@[inline] def front (s : Substring) : Char :=
+@[inline, expose] def front (s : Substring) : Char :=
   s.get 0
 
 @[export lean_substring_front]
@@ -2369,15 +3860,7 @@ theorem ext {s₁ s₂ : String} (h : s₁.data = s₂.data) : s₁ = s₂ :=
 @[simp]
 theorem String.mk_eq_asString (s : List Char) : String.mk s = List.asString s := rfl
 
-@[simp]
-theorem _root_.List.length_asString (s : List Char) : (List.asString s).length = s.length := by
-  rw [← length_data, List.data_asString]
-
 @[simp] theorem length_empty : "".length = 0 := by simp [← length_data, data_empty]
-
-@[simp]
-theorem bytes_singleton {c : Char} : (String.singleton c).bytes = [c].utf8Encode := by
-  simp [singleton]
 
 theorem singleton_eq {c : Char} : String.singleton c = [c].asString := by
   simp [← bytes_inj]
@@ -2390,10 +3873,10 @@ theorem length_singleton {c : Char} : (String.singleton c).length = 1 := by
   simp [← length_data]
 
 theorem push_eq_append (c : Char) : String.push s c = s ++ singleton c := by
-  simp [← bytes_inj]
+  simp
 
 @[simp] theorem data_push (c : Char) : (String.push s c).data = s.data ++ [c] := by
-  simp [push_eq_append]
+  simp [← append_singleton]
 
 @[simp] theorem length_push (c : Char) : (String.push s c).length = s.length + 1 := by
   simp [← length_data]
@@ -2410,18 +3893,11 @@ theorem lt_iff {s t : String} : s < t ↔ s.data < t.data := .rfl
 
 namespace Pos
 
-@[simp] theorem byteIdx_zero : (0 : Pos).byteIdx = 0 := rfl
-
 theorem byteIdx_mk (n : Nat) : byteIdx ⟨n⟩ = n := rfl
 
 @[simp] theorem mk_zero : ⟨0⟩ = (0 : Pos) := rfl
 
 @[simp] theorem mk_byteIdx (p : Pos) : ⟨p.byteIdx⟩ = p := rfl
-
-theorem ext {i₁ i₂ : Pos} (h : i₁.byteIdx = i₂.byteIdx) : i₁ = i₂ :=
-  show ⟨i₁.byteIdx⟩ = (⟨i₂.byteIdx⟩ : Pos) from h ▸ rfl
-
-theorem ext_iff {i₁ i₂ : Pos} : i₁ = i₂ ↔ i₁.byteIdx = i₂.byteIdx := ⟨fun h => h ▸ rfl, ext⟩
 
 @[simp] theorem add_byteIdx (p₁ p₂ : Pos) : (p₁ + p₂).byteIdx = p₁.byteIdx + p₂.byteIdx := rfl
 
@@ -2441,11 +3917,9 @@ theorem zero_addChar_byteIdx (c : Char) : ((0 : Pos) + c).byteIdx = c.utf8Size :
 theorem zero_addChar_eq (c : Char) : (0 : Pos) + c = ⟨c.utf8Size⟩ := by rw [← zero_addChar_byteIdx]
 
 theorem addChar_right_comm (p : Pos) (c₁ c₂ : Char) : p + c₁ + c₂ = p + c₂ + c₁ := by
-  apply ext
+  apply Pos.ext
   repeat rw [pos_add_char]
   apply Nat.add_right_comm
-
-theorem ne_of_lt {i₁ i₂ : Pos} (h : i₁ < i₂) : i₁ ≠ i₂ := mt ext_iff.1 (Nat.ne_of_lt h)
 
 theorem ne_of_gt {i₁ i₂ : Pos} (h : i₁ < i₂) : i₂ ≠ i₁ := (ne_of_lt h).symm
 
@@ -2466,16 +3940,7 @@ abbrev zero_addString_byteIdx := @byteIdx_zero_addString
 theorem zero_addString_eq (s : String) : (0 : Pos) + s = ⟨s.utf8ByteSize⟩ := by
   rw [← byteIdx_zero_addString]
 
-theorem le_iff {i₁ i₂ : Pos} : i₁ ≤ i₂ ↔ i₁.byteIdx ≤ i₂.byteIdx := .rfl
-
 @[simp] theorem mk_le_mk {i₁ i₂ : Nat} : Pos.mk i₁ ≤ Pos.mk i₂ ↔ i₁ ≤ i₂ := .rfl
-
-@[simp] theorem le_refl {p : Pos} : p ≤ p := mk_le_mk.mpr (Nat.le_refl _)
-
-@[simp] theorem le_trans {p1 p2 p3 : Pos} : p1 ≤ p2 → p2 ≤ p3 → p1 ≤ p3 := fun h1 h2 =>
-  mk_le_mk.mpr <| Nat.le_trans (mk_le_mk.mp h1) (mk_le_mk.mp h2)
-
-theorem lt_iff {i₁ i₂ : Pos} : i₁ < i₂ ↔ i₁.byteIdx < i₂.byteIdx := .rfl
 
 @[simp] theorem mk_lt_mk {i₁ i₂ : Nat} : Pos.mk i₁ < Pos.mk i₂ ↔ i₁ < i₂ := .rfl
 
@@ -2496,9 +3961,6 @@ theorem lt_next' (s : String) (p : Pos) : p < next s p := lt_next ..
 -- `toSubstring'` is just a synonym for `toSubstring` without the `@[inline]` attribute
 -- so for proving can be unfolded.
 attribute [simp] toSubstring'
-
-theorem append_assoc (s₁ s₂ s₃ : String) : (s₁ ++ s₂) ++ s₃ = s₁ ++ (s₂ ++ s₃) :=
-  ext (by simp [data_append])
 
 end String
 
